Support for atomic types.
Also finalizes some proofs.

rocq-bluerock-cpp2v/src/PrintType.cpp
@@ -199,6 +199,13 @@ public:
 		print.end_ctor();
 	}
 
+	void VisitAtomicType(const AtomicType* type, CoqPrinter& print,
+						 ClangPrinter& cprint) {
+		guard::ctor _{print, "Tatomic", false};
+		cprint.printQualType(print, type->getValueType(), loc::of(type));
+		print.end_ctor();
+	}
+
 	void VisitParenType(const ParenType* type, CoqPrinter& print,
 						ClangPrinter& cprint) {
 		cprint.printQualType(print, type->getInnerType(), loc::of(type));
