rocq-bluerock-brick/theories/lang/cpp/semantics/types.v
@@ -78,6 +78,7 @@ Fixpoint size_of (resolve : genv) (t : type) : option N :=
   | Tenum nm => glob_def resolve nm ≫= GlobDecl_size_of
   | Tfunction _ => None
   | Tbool => Some 1
+  | Tatomic _ => None
   | Tmember_pointer _ _ => None (* TODO these are not well supported right now *)
   | Tqualified _ t => size_of resolve t
   | Tnullptr => Some (pointer_size resolve)
